coq/LLVMGen/Correctness_AExpr.v
@@ -1,5 +1,6 @@
 Require Import Helix.LLVMGen.Correctness_Prelude.
 Require Import Helix.LLVMGen.Freshness.
+Require Import Helix.LLVMGen.LidBound.
 Require Import Helix.LLVMGen.Correctness_Invariants.
 Require Import Helix.LLVMGen.Correctness_NExpr.
 Require Import Helix.LLVMGen.Correctness_MExpr.
@@ -16,42 +17,20 @@ Opaque incLocal.
 
 Section AExpr.
 
-  Definition R_AExpr_start (σ : evalContext) (s : IRState) (memH : memoryH) (vellvm : memoryV * (local_env * global_env)) : Prop
-    := state_invariant σ s memH vellvm.
+  (* Definition R_AExpr_start (σ : evalContext) (s : IRState) (memH : memoryH) (vellvm : memoryV * (local_env * global_env)) : Prop *)
+  (*   := state_invariant σ s memH vellvm. *)
 
-  Definition R_AExpr
-             (σ : evalContext) (s : IRState)
-             (helix : memoryH * binary64)
-             (vellvm : memoryV * (local_env * res_L1)) : Prop
-    :=
-      let '(memH, b) := helix in
-      let '(memV, (ρ, (g, res))) := vellvm in
-      state_invariant σ s memH (memV, (ρ, g)) /\
-      res ≡ UVALUE_Double b.
+  (* Definition R_AExpr *)
+  (*            (σ : evalContext) (s : IRState) *)
+  (*            (helix : memoryH * binary64) *)
+  (*            (vellvm : memoryV * (local_env * res_L1)) : Prop *)
+  (*   := *)
+  (*     let '(memH, b) := helix in *)
+  (*     let '(memV, (ρ, (g, res))) := vellvm in *)
+  (*     state_invariant σ s memH (memV, (ρ, g)) /\ *)
+  (*     res ≡ UVALUE_Double b. *)
 
-  Hint Unfold R_AExpr: core.
-
-  (** ** Compilation of AExpr TODO
-   *)
-  Definition genAExpr_exp_correct (e: exp typ) : Rel_cfg_T binary64 unit :=
-    fun '(memH,i) '(memV,(l,(g,v))) =>
-      forall l', l ⊑ l' ->
-        interp_cfg (translate exp_E_to_instr_E (denote_exp (Some (DTYPE_Double)) (convert_typ [] e))) g l' memV
-        ≈
-        Ret (memV,(l',(g,UVALUE_Double i)))
-  .
-
-  Record genAExpr_rel
-         (σ : evalContext)
-         (aexp : AExpr)
-         (e : exp typ)
-         (mi : memoryH) (sti : config_cfg)
-         (mf : memoryH * binary64) (stf : config_cfg_T unit)
-    : Prop :=
-    {
-    aexp_correct : genAExpr_exp_correct e mf stf;
-    amonotone : ext_local mi sti mf stf
-    }.
+  (* Hint Unfold R_AExpr: core. *)
 
   (* TODO: move this *)
   Lemma int_of_nat :
@@ -187,9 +166,47 @@ Section AExpr.
     destruct a,b; try break_if; repeat break_match ;try reflexivity; crush.
   Qed.
 
-  Ltac split_post := split; [split | split]; cbn;
-                     [try solve_state_invariant | try solve_fresh | | intuition; try solve_sub_alist].
-  
+  Lemma state_invariant_incVoid :
+    forall σ s s' k memH stV,
+      incVoid s ≡ inr (s', k) ->
+      state_invariant σ s memH stV ->
+      state_invariant σ s' memH stV.
+  Proof.
+    intros * INC INV; inv INV.
+    split.
+    - red; repeat break_let; intros * LUH LUV.
+      erewrite incVoid_Γ in LUV; eauto.
+      generalize LUV; intros INLG;
+        eapply MINV in INLG; eauto.
+    - unfold WF_IRState; erewrite incVoid_Γ; eauto; apply WF.
+  Qed.
+
+  Definition genAExpr_exp_correct σ s1 s2 (e: exp typ) 
+    : Rel_cfg_T binary64 unit :=
+    fun '(x,i) '(memV,(l,(g,v))) =>
+      forall l',
+        local_scope_preserved s1 s2 l l' ->
+        Gamma_preserved σ s1 l l' ->
+        interp_cfg
+          (translate exp_E_to_instr_E (denote_exp (Some DTYPE_Double) (convert_typ [] e)))
+          g l' memV ≈
+          Ret (memV,(l',(g,UVALUE_Double i))).
+
+  Record genAExpr_post
+         (e : exp typ)
+         σ s1 s2
+         (mi : memoryH) (sti : config_cfg)
+         (mf : memoryH * binary64) (stf : config_cfg_T unit)
+    : Prop :=
+    {
+    exp_correct : genAExpr_exp_correct σ s1 s2 e mf stf;
+    is_almost_pure : almost_pure mi sti mf stf; 
+    extends : local_scope_modif s1 s2 (fst (snd sti)) (fst (snd stf));
+    exp_in_scope : forall id, e ≡ EXP_Ident (ID_Local id) -> ((exists v, alist_In id (fst (snd sti)) v) \/ (lid_bound_between s1 s2 id /\ s1 << s2));
+    Gamma_cst : Γ s2 ≡ Γ s1;
+    Mono_IRState : s1 << s2 \/ fst (snd sti) ≡ fst (snd stf)
+    }.
+
   Import ProofMode.
   Lemma genAExpr_correct :
     forall (* Compiler bits *) (s1 s2: IRState)
@@ -197,16 +214,18 @@ Section AExpr.
       (* Vellvm bits *)   (e: exp typ) (c: code typ) (g : global_env) (l : local_env) (memV : memoryV),
 
       genAExpr aexp s1 ≡ inr (s2, (e, c))      -> (* Compilation succeeds *)
-      state_invariant_pre σ s1 s2 memH (memV, (l, g)) -> (* The main state invariant is initially true *)
+      state_invariant σ s1 memH (memV, (l, g)) -> (* The main state invariant is initially true *)
+      Gamma_safe σ s1 s2 ->
       no_failure (interp_helix (E := E_cfg) (denoteAExpr σ aexp) memH) -> (* Source semantics defined *)
 
-      eutt (succ_cfg (lift_Rel_cfg (state_invariant_post σ s1 s2 l) ⩕ genAExpr_rel σ aexp e memH (mk_config_cfg memV l g)))
+      eutt (succ_cfg (lift_Rel_cfg (state_invariant σ s2) ⩕ genAExpr_post e σ s1 s2 memH (mk_config_cfg memV l g)))
            (interp_helix (denoteAExpr σ aexp) memH)
            (interp_cfg (denote_code (convert_typ [] c)) g l memV).
   Proof. 
-    intros s1 s2 aexp; revert s1 s2; induction aexp; intros * COMPILE [PRE PREF] NOFAIL.
+    intros s1 s2 aexp; revert s1 s2; induction aexp; intros * COMPILE PRE SAFE NOFAIL.
     - (* Variable case *)
       (* Reducing the compilation *)
+      pose proof PRE as PRE'; inv PRE'.
       cbn* in COMPILE; simp.
 
       + (* The variable maps to an integer in the IRState *)
@@ -222,12 +241,20 @@ Section AExpr.
 
         vstep.
         { vstep; eauto; reflexivity. }
-        apply eutt_Ret; split_post. 
-        red; intros.
-        cbn; vstep.
-        cbn; erewrite H; eauto.
-        eapply In_add_eq.
-        reflexivity.
+        apply eutt_Ret; split; [| split]; cbn; eauto.
+        * eapply state_invariant_add_fresh; eauto; split; eauto.
+        * intros l' LOC GAM; cbn*.
+          vstep; [ | reflexivity].
+          cbn.
+          red in LOC; rewrite LOC.
+          rewrite alist_find_add_eq; reflexivity.
+          eauto using lid_bound_between_incLocal.          
+        * apply local_scope_modif_add.
+          auto using lid_bound_between_incLocal.
+        * intros * EQ; inv EQ; right.
+          split; [auto using lid_bound_between_incLocal | solve_local_count].
+        * eauto using incLocal_Γ.
+        * left; solve_local_count.
 
       + (* The variable maps to a pointer *)
         unfold denoteAExpr in *; cbn* in *.
@@ -236,20 +263,28 @@ Section AExpr.
         break_match_goal; try_abs.
         clear NOFAIL.
         hvred.
-        apply eutt_Ret; split_post.
-        intros; break_match_goal; try_abs.
-        vstep.
-        eapply memory_invariant_LLU_AExpr; eauto;
-          eapply memory_invariant_ext_local;
-          eauto.
-        reflexivity.
+        apply eutt_Ret; split; [| split]; cbn; eauto.
+        * intros l' LOC GAM; cbn*.
+          break_match_goal; try_abs.
+          vstep.
+          red in GAM; cbn in *.
+          erewrite <- GAM.
+          eapply memory_invariant_LLU_AExpr; eauto.
+          econstructor;eauto.
+          reflexivity.
+        * intros * EQ; inv EQ.
+          left.
+          eexists.
+          eapply memory_invariant_LLU_AExpr; eauto.
 
     - (* Constant *)
       cbn* in *; simp.
       hvred.
-      apply eutt_Ret; split_post.
-      intros; vstep; reflexivity.
-      
+      apply eutt_Ret; split; [| split]; cbn; eauto.
+      intros l' MONO; cbn*.
+      vstep; reflexivity.
+      intros * EQ; inv EQ.
+
     - (* ANth m n: lookup to m[n] *)
 
       cbn* in *; simp.
@@ -259,19 +294,19 @@ Section AExpr.
       (* denoting [n] *)
       clean_goal.
       eapply eutt_clo_bind_returns; [eapply genNExpr_correct |..]; eauto.
-      split; cbn; auto; solve_fresh.
+      eapply Gamma_safe_shrink; eauto; solve_local_count.
+
       introR; destruct_unit.
       intros RET _; eapply no_failure_helix_bind_continuation in NOFAIL; [| eassumption]; clear RET.
-      destruct PRE0 as ([PRE1 PREF1] & EQEXP & ?).
+      destruct PRE0 as (SINV1 & POST1); inv POST1.
       cbn* in *; inv_eqs.
       hvred.
 
       (* denoting [m] *)
       eapply eutt_clo_bind_returns; [eapply genMExpr_correct | ..]; eauto.
-      split; auto; solve_fresh.
       introR; destruct_unit.
       intros RET _; eapply no_failure_helix_bind_continuation in NOFAIL; [| eassumption]; clear RET.
-      destruct vH0, PRE0 as ((PRE2 & PREF2) & ? & (addr_m & EQEXPm & LU_ARRAY)).
+      destruct vH0, PRE0 as (SINV2 & [PRES2 (addr_m & EQEXPm & LU_ARRAY) <-]). 
       cbn* in *; inv_eqs.
       hvred.
 
@@ -285,13 +320,14 @@ Section AExpr.
         [exact EQEXPm | | eapply LU_ARRAY; eauto |].
       { clear LU_ARRAY EQEXPm.
         assert (EQ: vH ≡ repr (Z.of_nat (MInt64asNT.to_nat vH))).
-        cbn.
-        unfold MInt64asNT.to_nat.
-        cbn.
-        rewrite Znat.Z2Nat.id, repr_intval; auto.
-        destruct (Int64.intrange vH); lia.
-        rewrite EQ in EQEXP.
-        exact EQEXP.
+        { cbn.
+          unfold MInt64asNT.to_nat.
+          cbn.
+          rewrite Znat.Z2Nat.id, repr_intval; auto.
+          destruct (Int64.intrange vH); lia.
+        }
+        rewrite EQ in exp_correct0.
+        apply exp_correct0; eauto using local_scope_preserved_refl, Gamma_preserved_refl.
       }
 
       rewrite EQ; clear EQ.
@@ -303,30 +339,51 @@ Section AExpr.
         apply lookup_alist_add_eq. 
         reflexivity.
       }
-      clear EQEXP EQEXPm NOFAIL.
-      apply eutt_Ret; split_post. 
-      * intros.
-        vstep.
-        solve_lu.
+
+      clear EQEXPm NOFAIL exp_correct0.
+      destruct u; clean_goal.
+      rename i0 into s2, i1 into s3, s2 into s4.
+      apply eutt_Ret; split; [| split]; cbn; eauto.
+      + eapply state_invariant_add_fresh; eauto.
+        eapply Gamma_safe_shrink; eauto.
+        rewrite <- Gamma_cst0; symmetry; eauto using incLocal_Γ.
+        solve_local_count.
+        solve_local_count.
+        eapply state_invariant_add_fresh; eauto.
+        eapply Gamma_safe_shrink; eauto.
+        solve_local_count.
+        solve_local_count.
+      + intros * SCO GAM.
+        vstep; eauto.
+        cbn.
+        erewrite SCO,alist_find_add_eq.
         reflexivity.
-      * (* Would be good to automate *)
-        etransitivity; eauto.
-        etransitivity; eauto.
-        apply sub_alist_add.
-        eapply freshness_pre_alist_fresh; eauto.
-        solve_fresh.
-        apply sub_alist_add.
-        eapply freshness_pre_alist_fresh; eauto.
-        solve_fresh.
-        
+        apply lid_bound_between_shrink_down with s3.
+        solve_local_count.
+        eapply lid_bound_between_incLocal; eauto.
+        reflexivity.
+      + eapply local_scope_modif_trans; eauto; [solve_local_count | solve_local_count |].
+        apply local_scope_modif_trans with (s2 := s3) (l2 := alist_add r (UVALUE_Addr x) l0).
+        solve_local_count.
+        solve_local_count.
+        eauto using local_scope_modif_add, lid_bound_between_incLocal.
+        eauto using local_scope_modif_add, lid_bound_between_incLocal.
+      + intros ? EQ; inv EQ.
+        right; split; [| solve_local_count].
+        apply lid_bound_between_shrink_down with s3; [solve_local_count |].
+        eauto using lid_bound_between_incLocal.
+      + rewrite <- Gamma_cst0.
+        etransitivity; eapply incLocal_Γ; eauto.
+      + left; solve_local_count.
+
     - (* AAbs *) 
       cbn* in *; simp.
       hvred.
       eapply eutt_clo_bind; try eapply IHaexp; eauto.
-      split; auto; solve_fresh.
+      eapply Gamma_safe_shrink; eauto; solve_local_count.
       introR; destruct_unit.
-      destruct PRE0 as ((PRE1 & PREF1) & AEXP & MONO).
-      cbn in MONO; inv_eqs.
+      destruct PRE0 as (SINV1 & [EXP1 EXT1 SCOPE1 VAR1 GAM1 MONO1]).
+      cbn in *; inv_eqs.
       cbn in *; hvred.
 
       (* TO FIX *)
@@ -335,7 +392,7 @@ Section AExpr.
       {
         cbn.
         vred_l.
-        rewrite (AEXP l0); [| reflexivity].
+        rewrite (EXP1 l0); eauto using local_scope_preserved_refl, Gamma_preserved_refl.
         tred; vred_l.
         reflexivity.
       }
@@ -344,228 +401,449 @@ Section AExpr.
         reflexivity.
       }
       reflexivity.
-      apply eutt_Ret; split_post.
-      * intros; vstep.
-        solve_lu.
+
+      clear EXP1 IHaexp.
+      clean_goal.
+      apply eutt_Ret; split; [| split]; cbn; eauto.
+      + eapply state_invariant_add_fresh; eauto.
+        eapply Gamma_safe_shrink; eauto.
+        solve_local_count.
+        solve_local_count.
+      + intros * SCO GAM.
+        vstep; eauto.
+        cbn.
+        erewrite SCO,alist_find_add_eq.
         reflexivity.
-      * (* Automate *)
-        etransitivity; eauto.
-        apply sub_alist_add.
-        eapply freshness_pre_alist_fresh; eauto.
-        solve_fresh.
-       
+        apply lid_bound_between_shrink_down with i.
+        solve_local_count.
+        eapply lid_bound_between_incLocal; eauto.
+        reflexivity.
+      + eapply local_scope_modif_trans; eauto; [solve_local_count | solve_local_count |].
+        eauto using local_scope_modif_add, lid_bound_between_incLocal.
+      + intros ? EQ; inv EQ.
+        right; split; [| solve_local_count].
+        apply lid_bound_between_shrink_down with i; [solve_local_count |].
+        eauto using lid_bound_between_incLocal.
+      + rewrite <- GAM1.
+        eapply incLocal_Γ; eauto.
+      + left; solve_local_count.
+        
     - (* APlus *)
       cbn* in *; simp...
       hvred.
 
       eapply eutt_clo_bind_returns; try eapply IHaexp1; eauto.
-      split; auto; solve_fresh.
+      eapply Gamma_safe_shrink; eauto; solve_local_count.
       introR; destruct_unit.
       intros RET _; eapply no_failure_helix_bind_continuation in NOFAIL; [| eassumption]; clear RET.
-      destruct PRE0 as ((PRE1 & PREF1) & AEXP1 & ext); cbn in *; inv_eqs.
+      destruct PRE0 as (SINV1 & [EXP1 EXT1 SCOPE1 VAR1 GAM1 MONO1]).
+      cbn in *; inv_eqs.
       cbn in *; hvred.
 
       eapply eutt_clo_bind; try eapply IHaexp2; eauto.
-      split; auto; solve_fresh.
+      eapply Gamma_safe_shrink; eauto; solve_local_count.
       introR; destruct_unit.
-      destruct PRE0 as ((PRE2 & PREF2) & AEXP2 & ext); cbn in *; inv_eqs.
+      destruct PRE0 as (SINV2 & [EXP2 EXT2 SCOPE2 VAR2 GAM2 MONO2]).
+      cbn in *; inv_eqs.
       hvred.
+
+      rename i into s2, i0 into s3, s2 into s4.
+      specialize (EXP1 l1) .
+      specialize (EXP2 l1) .
+      forward EXP2.
+      auto using local_scope_preserved_refl.
+      forward EXP2.
+      auto using Gamma_preserved_refl.
+      forward EXP1.
+      {
+        destruct MONO2 as [| <-]; [| apply local_scope_preserved_refl].
+        eapply local_scope_preserve_modif; eauto.
+      }
+      forward EXP1.
+      {
+        clear EXP2 EXP1 IHaexp2 IHaexp1.
+        clean_goal.
+        apply Gamma_preserved_Gamma_eq with s2; auto.
+        eapply Gamma_preserved_if_safe; eauto.
+        eapply Gamma_safe_shrink; eauto; solve_local_count.
+      }
 
       vstep.
       {
-        vstep.
-        rewrite AEXP1; auto; reflexivity.
-        rewrite AEXP2; auto; reflexivity.
+        vstep; eauto.
         all:reflexivity.
       }
 
-      apply eutt_Ret; split_post.
-      * intros; vstep.
-        solve_lu.
+      apply eutt_Ret; split; [| split]; cbn; eauto.
+      + eapply state_invariant_add_fresh; eauto.
+        eapply Gamma_safe_shrink; eauto. rewrite GAM2; auto.
+        solve_local_count.
+        solve_local_count.
+      + intros * SCO GAM.
+        vstep; eauto.
+        cbn.
+        erewrite SCO,alist_find_add_eq.
         reflexivity.
-      * (* Automate *)
-        etransitivity; eauto.
-        etransitivity; eauto.
-        apply sub_alist_add.
-        eapply freshness_pre_alist_fresh; eauto.
-        solve_fresh.
+        apply lid_bound_between_shrink_down with s3.
+        solve_local_count.
+        eapply lid_bound_between_incLocal; eauto.
+        reflexivity.
+      + eapply local_scope_modif_trans; eauto; [solve_local_count | solve_local_count |].
+        eapply local_scope_modif_trans; eauto; [solve_local_count | solve_local_count |].
+        eauto using local_scope_modif_add, lid_bound_between_incLocal.
+      + intros ? EQ; inv EQ.
+        right; split; [| solve_local_count].
+        apply lid_bound_between_shrink_down with s3; [solve_local_count |].
+        eauto using lid_bound_between_incLocal.
+      + rewrite <- GAM1, <- GAM2.
+        eapply incLocal_Γ; eauto.
+      + left; solve_local_count.
 
     - (* AMinus *)
       cbn* in *; simp.
       hvred.
 
       eapply eutt_clo_bind_returns; try eapply IHaexp1; eauto.
-      split; auto; solve_fresh.
+      eapply Gamma_safe_shrink; eauto; solve_local_count.
       introR; destruct_unit.
       intros RET _; eapply no_failure_helix_bind_continuation in NOFAIL; [| eassumption]; clear RET.
-      destruct PRE0 as ((PRE1 & PREF1) & AEXP1 & ext); cbn in *; inv_eqs.
+      destruct PRE0 as (SINV1 & [EXP1 EXT1 SCOPE1 VAR1 GAM1 MONO1]).
+      cbn in *; inv_eqs.
       hvred.
 
       eapply eutt_clo_bind; try eapply IHaexp2; eauto.
-      split; auto; solve_fresh.
+      eapply Gamma_safe_shrink; eauto; solve_local_count.
       introR; destruct_unit.
-      destruct PRE0 as ((PRE2 & PREF2) & AEXP2 & ext); cbn in *; inv_eqs.
+      destruct PRE0 as (SINV2 & [EXP2 EXT2 SCOPE2 VAR2 GAM2 MONO2]).
+      cbn in *; inv_eqs.
       hvred.
+
+      rename i into s2, i0 into s3, s2 into s4.
+      specialize (EXP1 l1) .
+      specialize (EXP2 l1) .
+      forward EXP2.
+      auto using local_scope_preserved_refl.
+      forward EXP2.
+      auto using Gamma_preserved_refl.
+      forward EXP1.
+      {
+        destruct MONO2 as [| <-]; [| apply local_scope_preserved_refl].
+        eapply local_scope_preserve_modif; eauto.
+      }
+      forward EXP1.
+      {
+        clear EXP2 EXP1 IHaexp2 IHaexp1.
+        clean_goal.
+        apply Gamma_preserved_Gamma_eq with s2; auto.
+        eapply Gamma_preserved_if_safe; eauto.
+        eapply Gamma_safe_shrink; eauto; solve_local_count.
+      }
 
       vstep.
       {
-        vstep.
-        rewrite AEXP1; auto; reflexivity.
-        rewrite AEXP2; auto; reflexivity. 
+        vstep; eauto.
         all:reflexivity.
       }
 
-      apply eutt_Ret; split_post.
-      * intros; vstep.
-        solve_lu.
+      apply eutt_Ret; split; [| split]; cbn; eauto.
+      + eapply state_invariant_add_fresh; eauto.
+        eapply Gamma_safe_shrink; eauto. rewrite GAM2; auto.
+        solve_local_count.
+        solve_local_count.
+      + intros * SCO GAM.
+        vstep; eauto.
+        cbn.
+        erewrite SCO,alist_find_add_eq.
         reflexivity.
-      * (* Automate *)
-        etransitivity; eauto.
-        etransitivity; eauto.
-        apply sub_alist_add.
-        eapply freshness_pre_alist_fresh; eauto.
-        solve_fresh.
+        apply lid_bound_between_shrink_down with s3.
+        solve_local_count.
+        eapply lid_bound_between_incLocal; eauto.
+        reflexivity.
+      + eapply local_scope_modif_trans; eauto; [solve_local_count | solve_local_count |].
+        eapply local_scope_modif_trans; eauto; [solve_local_count | solve_local_count |].
+        eauto using local_scope_modif_add, lid_bound_between_incLocal.
+      + intros ? EQ; inv EQ.
+        right; split; [| solve_local_count].
+        apply lid_bound_between_shrink_down with s3; [solve_local_count |].
+        eauto using lid_bound_between_incLocal.
+      + rewrite <- GAM1, <- GAM2.
+        eapply incLocal_Γ; eauto.
+      + left; solve_local_count.
 
     - (* AMult *)
       cbn* in *; simp.
       hvred.
 
       eapply eutt_clo_bind_returns; try eapply IHaexp1; eauto.
-      split; auto; solve_fresh.
+      eapply Gamma_safe_shrink; eauto; solve_local_count.
       introR; destruct_unit.
       intros RET _; eapply no_failure_helix_bind_continuation in NOFAIL; [| eassumption]; clear RET.
-      destruct PRE0 as ((PRE1 & PREF1) & AEXP1 & ext); cbn in *; inv_eqs.
+      destruct PRE0 as (SINV1 & [EXP1 EXT1 SCOPE1 VAR1 GAM1 MONO1]).
+      cbn in *; inv_eqs.
       hvred.
 
       eapply eutt_clo_bind; try eapply IHaexp2; eauto.
-      split; auto; solve_fresh.
+      eapply Gamma_safe_shrink; eauto; solve_local_count.
       introR; destruct_unit.
-      destruct PRE0 as ((PRE2 & PREF2) & AEXP2 & ext); cbn in *; inv_eqs.
+      destruct PRE0 as (SINV2 & [EXP2 EXT2 SCOPE2 VAR2 GAM2 MONO2]).
+      cbn in *; inv_eqs.
       hvred.
+
+      rename i into s2, i0 into s3, s2 into s4.
+      specialize (EXP1 l1) .
+      specialize (EXP2 l1) .
+      forward EXP2.
+      auto using local_scope_preserved_refl.
+      forward EXP2.
+      auto using Gamma_preserved_refl.
+      forward EXP1.
+      {
+        destruct MONO2 as [| <-]; [| apply local_scope_preserved_refl].
+        eapply local_scope_preserve_modif; eauto.
+      }
+      forward EXP1.
+      {
+        clear EXP2 EXP1 IHaexp2 IHaexp1.
+        clean_goal.
+        apply Gamma_preserved_Gamma_eq with s2; auto.
+        eapply Gamma_preserved_if_safe; eauto.
+        eapply Gamma_safe_shrink; eauto; solve_local_count.
+      }
 
       vstep.
       {
-        vstep.
-        rewrite AEXP1; auto; reflexivity.
-        rewrite AEXP2; auto; reflexivity.
+        vstep; eauto.
         all:reflexivity.
       }
 
-      apply eutt_Ret; split_post.
-      * intros; vstep.
-        solve_lu.
+      apply eutt_Ret; split; [| split]; cbn; eauto.
+      + eapply state_invariant_add_fresh; eauto.
+        eapply Gamma_safe_shrink; eauto. rewrite GAM2; auto.
+        solve_local_count.
+        solve_local_count.
+      + intros * SCO GAM.
+        vstep; eauto.
+        cbn.
+        erewrite SCO,alist_find_add_eq.
         reflexivity.
-      * (* Automate *)
-        etransitivity; eauto.
-        etransitivity; eauto.
-        apply sub_alist_add.
-        eapply freshness_pre_alist_fresh; eauto.
-        solve_fresh.
+        apply lid_bound_between_shrink_down with s3.
+        solve_local_count.
+        eapply lid_bound_between_incLocal; eauto.
+        reflexivity.
+      + eapply local_scope_modif_trans; eauto; [solve_local_count | solve_local_count |].
+        eapply local_scope_modif_trans; eauto; [solve_local_count | solve_local_count |].
+        eauto using local_scope_modif_add, lid_bound_between_incLocal.
+      + intros ? EQ; inv EQ.
+        right; split; [| solve_local_count].
+        apply lid_bound_between_shrink_down with s3; [solve_local_count |].
+        eauto using lid_bound_between_incLocal.
+      + rewrite <- GAM1, <- GAM2.
+        eapply incLocal_Γ; eauto.
+      + left; solve_local_count.
 
     - (* AMin *)
       cbn* in *; simp.
       hvred.
 
       eapply eutt_clo_bind_returns; try eapply IHaexp1; eauto.
-      split; auto; solve_fresh.
+      eapply Gamma_safe_shrink; eauto; solve_local_count.
       introR; destruct_unit.
       intros RET _; eapply no_failure_helix_bind_continuation in NOFAIL; [| eassumption]; clear RET.
-      destruct PRE0 as ((PRE1 & PREF1) & AEXP1 & ext); cbn in *; inv_eqs.
+      destruct PRE0 as (SINV1 & [EXP1 EXT1 SCOPE1 VAR1 GAM1 MONO1]).
+      cbn in *; inv_eqs.
       hvred.
 
       eapply eutt_clo_bind; try eapply IHaexp2; eauto.
-      split; auto; solve_fresh.
+      eapply Gamma_safe_shrink; eauto; solve_local_count.
       introR; destruct_unit.
-      destruct PRE0 as ((PRE2 & PREF2) & AEXP2 & ext); cbn in *; inv_eqs.
+      destruct PRE0 as (SINV2 & [EXP2 EXT2 SCOPE2 VAR2 GAM2 MONO2]).
+      cbn in *; inv_eqs.
       hvred.
+
+      rename i into s2, i0 into s3, s2 into s4.
+      specialize (EXP1 l1) .
+      specialize (EXP2 l1) .
+      forward EXP2.
+      auto using local_scope_preserved_refl.
+      forward EXP2.
+      auto using Gamma_preserved_refl.
+      forward EXP1.
+      {
+        destruct MONO2 as [| <-]; [| apply local_scope_preserved_refl].
+        eapply local_scope_preserve_modif; eauto.
+      }
+      forward EXP1.
+      {
+        clear EXP2 EXP1 IHaexp2 IHaexp1.
+        clean_goal.
+        apply Gamma_preserved_Gamma_eq with s2; auto.
+        eapply Gamma_preserved_if_safe; eauto.
+        eapply Gamma_safe_shrink; eauto; solve_local_count.
+      }
 
       vstep; try reflexivity.
       { cbn; vred_l. 
-        rewrite AEXP1; auto.
+        rewrite EXP1.
         autorewrite with itree.
         vred_l.
-        rewrite AEXP2; auto. 
+        rewrite EXP2.
         autorewrite with itree.
         vred_l.
-        reflexivity.
         reflexivity.
       }
       cbn; tred; vred_l; reflexivity.
       reflexivity.
 
-      apply eutt_Ret; split_post.
-      * intros; vstep.
-        solve_lu.
-        rewrite min_float_correct.
+      apply eutt_Ret; split; [| split]; cbn; eauto.
+      + eapply state_invariant_add_fresh; eauto.
+        eapply Gamma_safe_shrink; eauto. rewrite GAM2; auto.
+        solve_local_count.
+        solve_local_count.
+      + intros * SCO GAM.
+        vstep; eauto.
+        cbn.
+        erewrite SCO,alist_find_add_eq.
         reflexivity.
-      * (* Automate *)
-        etransitivity; eauto.
-        etransitivity; eauto.
-        apply sub_alist_add.
-        eapply freshness_pre_alist_fresh; eauto.
-        solve_fresh.
+        apply lid_bound_between_shrink_down with s3.
+        solve_local_count.
+        eapply lid_bound_between_incLocal; eauto.
+        rewrite min_float_correct. 
+        reflexivity.
+      + eapply local_scope_modif_trans; eauto; [solve_local_count | solve_local_count |].
+        eapply local_scope_modif_trans; eauto; [solve_local_count | solve_local_count |].
+        eauto using local_scope_modif_add, lid_bound_between_incLocal.
+      + intros ? EQ; inv EQ.
+        right; split; [| solve_local_count].
+        apply lid_bound_between_shrink_down with s3; [solve_local_count |].
+        eauto using lid_bound_between_incLocal.
+      + rewrite <- GAM1, <- GAM2.
+        eapply incLocal_Γ; eauto.
+      + left; solve_local_count.
         
    - (* AMax *)
       cbn* in *; simp.
       hvred.
 
       eapply eutt_clo_bind_returns; try eapply IHaexp1; eauto.
-      split; auto; solve_fresh.
+      eapply Gamma_safe_shrink; eauto; solve_local_count.
       introR; destruct_unit.
       intros RET _; eapply no_failure_helix_bind_continuation in NOFAIL; [| eassumption]; clear RET.
-      destruct PRE0 as ((PRE1 & PREF1) & AEXP1 & ext); cbn in *; inv_eqs.
+      destruct PRE0 as (SINV1 & [EXP1 EXT1 SCOPE1 VAR1 GAM1 MONO1]).
+      cbn in *; inv_eqs.
       hvred.
 
       eapply eutt_clo_bind; try eapply IHaexp2; eauto.
-      split; auto; solve_fresh.
+      eapply Gamma_safe_shrink; eauto; solve_local_count.
       introR; destruct_unit.
-      destruct PRE0 as ((PRE2 & PREF2) & AEXP2 & ext); cbn in *; inv_eqs.
+      destruct PRE0 as (SINV2 & [EXP2 EXT2 SCOPE2 VAR2 GAM2 MONO2]).
+      cbn in *; inv_eqs.
       hvred.
 
-      vstep.
-      { cbn; tred; vred_l.
-        rewrite AEXP1; eauto.
-        tred; vred_l; rewrite AEXP2.
-        tred; vred_l; reflexivity.
+      rename i into s2, i0 into s3, s2 into s4.
+      specialize (EXP1 l1) .
+      specialize (EXP2 l1) .
+      forward EXP2.
+      auto using local_scope_preserved_refl.
+      forward EXP2.
+      auto using Gamma_preserved_refl.
+      forward EXP1.
+      {
+        destruct MONO2 as [| <-]; [| apply local_scope_preserved_refl].
+        eapply local_scope_preserve_modif; eauto.
+      }
+      forward EXP1.
+      {
+        clear EXP2 EXP1 IHaexp2 IHaexp1.
+        clean_goal.
+        apply Gamma_preserved_Gamma_eq with s2; auto.
+        eapply Gamma_preserved_if_safe; eauto.
+        eapply Gamma_safe_shrink; eauto; solve_local_count.
+      }
+
+      vstep; try reflexivity.
+      { cbn; vred_l. 
+        rewrite EXP1.
+        autorewrite with itree.
+        vred_l.
+        rewrite EXP2.
+        autorewrite with itree.
+        vred_l.
         reflexivity.
       }
       cbn; tred; vred_l; reflexivity.
       reflexivity.
 
-      apply eutt_Ret; split_post.
-      * intros; vstep.
-        solve_lu.
-        rewrite max_float_correct.
+      apply eutt_Ret; split; [| split]; cbn; eauto.
+      + eapply state_invariant_add_fresh; eauto.
+        eapply Gamma_safe_shrink; eauto. rewrite GAM2; auto.
+        solve_local_count.
+        solve_local_count.
+      + intros * SCO GAM.
+        vstep; eauto.
+        cbn.
+        erewrite SCO,alist_find_add_eq.
         reflexivity.
-      * (* Automate *)
-        etransitivity; eauto.
-        etransitivity; eauto.
-        apply sub_alist_add.
-        eapply freshness_pre_alist_fresh; eauto.
-        solve_fresh.
-
+        apply lid_bound_between_shrink_down with s3.
+        solve_local_count.
+        eapply lid_bound_between_incLocal; eauto.
+        rewrite max_float_correct. 
+        reflexivity.
+      + eapply local_scope_modif_trans; eauto; [solve_local_count | solve_local_count |].
+        eapply local_scope_modif_trans; eauto; [solve_local_count | solve_local_count |].
+        eauto using local_scope_modif_add, lid_bound_between_incLocal.
+      + intros ? EQ; inv EQ.
+        right; split; [| solve_local_count].
+        apply lid_bound_between_shrink_down with s3; [solve_local_count |].
+        eauto using lid_bound_between_incLocal.
+      + rewrite <- GAM1, <- GAM2.
+        eapply incLocal_Γ; eauto.
+      + left; solve_local_count.
+ 
    - (* AZless *)
       cbn* in *; simp.
       hvred.
 
       eapply eutt_clo_bind_returns; try eapply IHaexp1; eauto.
-      split; auto; solve_fresh.
+      eapply Gamma_safe_shrink; eauto; solve_local_count.
       introR; destruct_unit.
       intros RET _; eapply no_failure_helix_bind_continuation in NOFAIL; [| eassumption]; clear RET.
-      destruct PRE0 as ((PRE1 & PREF1) & AEXP1 & ext); cbn in *; inv_eqs.
+      destruct PRE0 as (SINV1 & [EXP1 EXT1 SCOPE1 VAR1 GAM1 MONO1]).
+      cbn in *; inv_eqs.
       hvred.
 
       eapply eutt_clo_bind; try eapply IHaexp2; eauto.
-      split; auto; solve_fresh.
+      eapply Gamma_safe_shrink; eauto; solve_local_count.
       introR; destruct_unit.
-      destruct PRE0 as ((PRE2 & PREF2) & AEXP2 & ext); cbn in *; inv_eqs.
+      destruct PRE0 as (SINV2 & [EXP2 EXT2 SCOPE2 VAR2 GAM2 MONO2]).
+      cbn in *; inv_eqs.
       hvred.
+
+      rename i into s2, i0 into s3, s2 into s4.
+      specialize (EXP1 l1) .
+      specialize (EXP2 l1) .
+      forward EXP2.
+      auto using local_scope_preserved_refl.
+      forward EXP2.
+      auto using Gamma_preserved_refl.
+      forward EXP1.
+      {
+        destruct MONO2 as [| <-]; [| apply local_scope_preserved_refl].
+        eapply local_scope_preserve_modif; eauto.
+      }
+      forward EXP1.
+      {
+        clear EXP2 EXP1 IHaexp2 IHaexp1.
+        clean_goal.
+        apply Gamma_preserved_Gamma_eq with s2; auto.
+        eapply Gamma_preserved_if_safe; eauto.
+        eapply Gamma_safe_shrink; eauto; solve_local_count.
+      }
 
       vstep.
       {
         vstep.
-        rewrite AEXP1; auto; reflexivity.
-        rewrite AEXP2; auto; reflexivity. 
+        rewrite EXP1; reflexivity.
+        rewrite EXP2; reflexivity. 
         all: reflexivity.
       }
 
@@ -586,39 +864,56 @@ Section AExpr.
       cbn; match_rewrite; reflexivity.
       reflexivity.
 
-      apply eutt_Ret. split; [split | split].
-      {
-        eapply state_invariant_incVoid; [eauto | ..].
+      clear EXP1 EXP2 NOFAIL IHaexp1 IHaexp2.
+      clean_goal.
+      rename i1 into s4, i2 into s5, s4 into s6.
+      
+      apply eutt_Ret; split; [| split]; cbn; eauto.
+      + eapply state_invariant_incVoid; [eauto | ..].
         eapply state_invariant_add_fresh; [eauto |..].
-        eapply state_invariant_add_fresh; [eauto | eauto | solve_fresh].
-        eapply freshness_pre_incLocal; [eassumption | ].
-        solve_fresh.
-      }
-      {
+        eapply Gamma_safe_shrink; eauto.
+        rewrite <- GAM1, <- GAM2; auto.
+        symmetry; eapply incLocal_Γ; eauto.
+        solve_local_count.
+        solve_local_count.
+        eapply state_invariant_add_fresh; [eauto |..].
+        eapply Gamma_safe_shrink; eauto.
+        rewrite <- GAM1, <- GAM2; auto.
+        solve_local_count.
+        solve_local_count.
+        auto.
+      + intros * SCO GAM.
+        vstep; eauto.
         cbn.
-        eapply freshness_post_incVoid; eauto.
-        solve_fresh.
-      }
-      {
-        cbn; intros.
-        vstep.
-        solve_lu.
-        rewrite H2.
+        erewrite SCO,alist_find_add_eq.
         reflexivity.
-      }
-      {
-        cbn; intuition.
-        etransitivity; eauto.
-        etransitivity; eauto.
-        etransitivity.
-        apply sub_alist_add.
-        2:apply sub_alist_add.
-        eapply freshness_pre_alist_fresh; [| eassumption].
-        solve_fresh.
-        eapply freshness_pre_alist_fresh; [| eassumption].
-        eapply freshness_pre_incLocal; [eassumption | ].
-        solve_fresh.
-      }
-Qed.
+        apply lid_bound_between_shrink_down with s4.
+        solve_local_count.
+        apply lid_bound_between_shrink_up with s5.
+        solve_local_count.
+        eapply lid_bound_between_incLocal; eauto.
+        rewrite H0; reflexivity.
+      + eapply local_scope_modif_trans; eauto; [solve_local_count | solve_local_count |].
+        eapply local_scope_modif_trans; eauto; [solve_local_count | solve_local_count |].
+        apply local_scope_modif_trans
+          with (s2 := s4) (l2 := alist_add r (dvalue_to_uvalue (double_cmp FOlt vH vH0)) l1); [solve_local_count | solve_local_count | |].
+        eauto using local_scope_modif_add, lid_bound_between_incLocal.
+        apply local_scope_modif_trans with
+            (s2 := s5)
+            (l2 := alist_add r0 (UVALUE_Double (Floats.Float.of_longu (DynamicValues.Int64.repr (DynamicValues.Int1.unsigned x)))) (alist_add r (dvalue_to_uvalue (double_cmp FOlt vH vH0)) l1))
+        ; [solve_local_count | solve_local_count | |].
+        eauto using local_scope_modif_add, lid_bound_between_incLocal.
+        eapply local_scope_modif_refl.
+      + intros ? EQ; inv EQ.
+        right; split; [| solve_local_count].
+        apply lid_bound_between_shrink_down with s4; [solve_local_count |].
+        apply lid_bound_between_shrink_up with s5; [solve_local_count |].
+        eauto using lid_bound_between_incLocal.
+      + rewrite <- GAM1, <- GAM2.
+        apply incLocal_Γ in Heqs1; rewrite <- Heqs1.
+        apply incLocal_Γ in Heqs2; rewrite <- Heqs2.
+        apply incVoid_Γ in Heqs3; auto. 
+      + left; solve_local_count.
+  Qed.
 
 End AExpr.
